fstar/MLS.Symbolic.Parsers.fst
@@ -1,0 +1,46 @@
+module MLS.Symbolic.Parsers
+
+open Comparse
+open MLS.Tree
+
+#set-options "--fuel 1 --ifuel 1"
+
+noeq type tree_internal_node (bytes:Type0) {|bytes_like bytes|} (leaf_t:Type0) (node_t:Type0) (l:pos) (i:tree_index l) (ps_node_t:parser_serializer_unit bytes node_t) (ps_left:parser_serializer bytes (tree leaf_t node_t (l-1) (left_index i))) (ps_right:parser_serializer bytes (tree leaf_t node_t (l-1) (right_index i))) = {
+  [@@@ with_parser #bytes ps_left]
+  left: tree leaf_t node_t (l-1) (left_index i);
+  [@@@ with_parser #bytes ps_node_t]
+  data: node_t;
+  [@@@ with_parser #bytes ps_right]
+  right: tree leaf_t node_t (l-1) (right_index i);
+}
+
+%splice [ps_tree_internal_node] (gen_parser (`tree_internal_node))
+%splice [ps_tree_internal_node_is_valid] (gen_is_valid_lemma (`tree_internal_node))
+
+[@@"opaque_to_smt"]
+val ps_tree: #bytes:Type0 -> {|bytes_like bytes|} -> #leaf_t:Type0 -> #node_t:Type0 -> parser_serializer bytes leaf_t -> parser_serializer_unit bytes node_t -> l:nat -> i:tree_index l -> parser_serializer bytes (tree leaf_t node_t l i)
+let rec ps_tree #bytes #bl #leaf_t #node_t ps_leaf_t ps_node_t l i =
+  if l = 0 then (
+    mk_isomorphism
+      (tree leaf_t node_t 0 i)
+      ps_leaf_t
+      (fun x -> TLeaf x)
+      (fun (TLeaf x) -> x)
+  ) else (
+    mk_isomorphism
+      (tree leaf_t node_t l i)
+      (ps_tree_internal_node #bytes #bl leaf_t node_t l i ps_node_t (ps_tree ps_leaf_t ps_node_t (l-1) (left_index i)) (ps_tree ps_leaf_t ps_node_t (l-1) (right_index i)))
+      (fun {left; data; right} -> TNode data left right)
+      (fun (TNode data left right) -> {left; data; right})
+  )
+
+val ps_tree_is_valid: #bytes:Type0 -> {|bytes_like bytes|} -> #leaf_t:Type0 -> #node_t:Type0 -> ps_leaf_t:parser_serializer bytes leaf_t -> ps_node_t:parser_serializer_unit bytes node_t -> l:nat -> i:tree_index l -> pre:bytes_compatible_pre bytes -> x:tree leaf_t node_t l i -> Lemma
+  ((ps_tree ps_leaf_t ps_node_t l i).is_valid pre x <==> (
+    match x with
+    | TLeaf y -> ps_leaf_t.is_valid pre y
+    | TNode y left right -> ps_node_t.is_valid pre y /\ (ps_tree ps_leaf_t ps_node_t (l-1) (left_index i)).is_valid pre left /\ (ps_tree ps_leaf_t ps_node_t (l-1) (right_index i)).is_valid pre right
+  ))
+  [SMTPat ((ps_tree ps_leaf_t ps_node_t l i).is_valid pre x)]
+let ps_tree_is_valid #bytes #bl #leaf_t #node_t ps_leaf_t ps_node_t l i pre x =
+  // For some reason, reveal_opaque doesn't work here
+  normalize_term_spec (ps_tree ps_leaf_t ps_node_t l i)
