fstar/MLS.TreeSync.Symbolic.API.Sessions.fst
@@ -1,0 +1,286 @@
+module MLS.TreeSync.Symbolic.API.Sessions
+
+open Comparse
+open GlobalRuntimeLib
+open LabeledRuntimeAPI
+open MLS.Tree
+open MLS.NetworkTypes
+open MLS.TreeSync.NetworkTypes
+open MLS.TreeSync.Types
+open MLS.TreeSync.Invariants.UnmergedLeaves
+open MLS.TreeSync.Invariants.ParentHash
+open MLS.TreeSync.Invariants.ValidLeaves
+open MLS.TreeSync.Invariants.AuthService
+open MLS.TreeSync.API.Types
+open MLS.Symbolic
+open MLS.Symbolic.Sessions
+open MLS.Symbolic.Parsers
+open MLS.TreeSync.Symbolic.IsValid
+open MLS.TreeSync.Symbolic.SignatureGuarantees
+
+#set-options "--fuel 1 --ifuel 1"
+
+(*** Session predicate for public state ***)
+
+val ps_treesync: #bytes:Type0 -> {|bytes_like bytes|} -> tkt:treekem_types bytes -> l:nat -> i:tree_index l -> parser_serializer bytes (treesync bytes tkt l i)
+let ps_treesync #bytes tkt l i =
+  ps_tree (ps_option (ps_leaf_node_nt tkt)) (ps_option (ps_parent_node_nt tkt)) l i
+
+val ps_treesync_is_valid: #bytes:Type0 -> {|bytes_like bytes|} -> tkt:treekem_types bytes -> l:nat -> i:tree_index l -> pre:bytes_compatible_pre bytes -> x:treesync bytes tkt l i -> Lemma
+  ((ps_treesync tkt l i).is_valid pre x <==> treesync_has_pre pre x)
+let rec ps_treesync_is_valid #bytes #bl tkt l i pre x =
+  match x with
+  | TLeaf _ -> ()
+  | TNode data left right ->
+    ps_treesync_is_valid tkt (l-1) (left_index i) pre left;
+    ps_treesync_is_valid tkt (l-1) (right_index i) pre right
+
+val ps_as_tokens: #bytes:Type0 -> {|bytes_like bytes|} -> #as_token:Type0 -> parser_serializer bytes as_token -> l:nat -> i:tree_index l -> parser_serializer bytes (as_tokens bytes as_token l i)
+let ps_as_tokens #bytes #bl #as_token ps_token l i =
+  ps_tree (ps_option ps_token) ps_unit l i
+
+val ps_dy_as_tokens: l:nat -> i:tree_index l -> parser_serializer dy_bytes (as_tokens dy_bytes dy_as_token l i)
+let ps_dy_as_tokens l i =
+  ps_as_tokens ps_dy_as_token l i
+
+#push-options "--z3rlimit 25"
+val ps_dy_as_tokens_is_valid: #l:nat -> #i:tree_index l -> pre:bytes_compatible_pre dy_bytes -> tokens:as_tokens dy_bytes dy_as_token l i ->
+  Lemma ((ps_dy_as_tokens l i).is_valid pre tokens)
+let rec ps_dy_as_tokens_is_valid #l #i pre tokens =
+  match tokens with
+  | TLeaf x -> (
+    match x with
+    | None -> ()
+    | Some y -> ()
+  )
+  | TNode _ left right ->
+    ps_dy_as_tokens_is_valid pre left;
+    ps_dy_as_tokens_is_valid pre right
+#pop-options
+
+noeq
+type bare_treesync_state_ (bytes:Type0) {|bytes_like bytes|} (tkt:treekem_types bytes) (as_token:Type0) (ps_token:parser_serializer bytes as_token) = {
+  group_id: mls_bytes bytes;
+  [@@@ with_parser #bytes ps_nat]
+  levels: nat;
+  [@@@ with_parser #bytes (ps_treesync tkt levels 0)]
+  tree: treesync bytes tkt levels 0;
+  [@@@ with_parser #bytes (ps_as_tokens ps_token levels 0)]
+  tokens: as_tokens bytes as_token levels 0;
+}
+
+%splice [ps_bare_treesync_state_] (gen_parser (`bare_treesync_state_))
+%splice [ps_bare_treesync_state__is_valid] (gen_is_valid_lemma (`bare_treesync_state_))
+
+type bare_treesync_state (tkt:treekem_types dy_bytes) =
+  bare_treesync_state_ dy_bytes tkt dy_as_token ps_dy_as_token
+
+instance parseable_serializeable_bare_treesync_state (tkt:treekem_types dy_bytes): parseable_serializeable dy_bytes (bare_treesync_state tkt) = mk_parseable_serializeable (ps_bare_treesync_state_ tkt dy_as_token ps_dy_as_token)
+
+val treesync_public_state_label: string
+let treesync_public_state_label = "MLS.TreeSync.PublicState"
+
+val bare_treesync_public_state_invariant: tkt:treekem_types dy_bytes -> bare_session_pred
+let bare_treesync_public_state_invariant tkt gu p time si vi session =
+  match parse (bare_treesync_state tkt) session with
+  | None -> False
+  | Some st -> (
+    is_publishable gu time st.group_id /\
+    treesync_has_pre (is_publishable gu time) st.tree /\
+    unmerged_leaves_ok st.tree /\
+    parent_hash_invariant st.tree /\
+    valid_leaves_invariant st.group_id st.tree /\
+    all_credentials_ok st.tree (st.tokens <: as_tokens dy_bytes (dy_asp gu time).token_t st.levels 0)
+  )
+
+#push-options "--fuel 0 --ifuel 0"
+val treesync_public_state_invariant: treekem_types dy_bytes -> session_pred
+let treesync_public_state_invariant tkt =
+  mk_session_pred (bare_treesync_public_state_invariant tkt)
+    (fun gu p time0 time1 si vi session ->
+      let st = Some?.v (parse (bare_treesync_state tkt) session) in
+      // Prove publishability of treesync in the future
+      ps_treesync_is_valid tkt st.levels 0 (is_publishable gu time0) st.tree;
+      ps_treesync_is_valid tkt st.levels 0 (is_publishable gu time1) st.tree;
+      MLS.MiscLemmas.comparse_is_valid_weaken (ps_treesync tkt st.levels 0) (is_publishable gu time0) (is_publishable gu time1) st.tree
+    )
+    (fun gu p time si vi session ->
+      let st = Some?.v (parse (bare_treesync_state tkt) session) in
+      let pre = is_msg gu (readers [psv_id p si vi]) time in
+      ps_treesync_is_valid tkt st.levels 0 (is_publishable gu time) st.tree;
+      MLS.MiscLemmas.comparse_is_valid_weaken (ps_treesync tkt st.levels 0) (is_publishable gu time) pre st.tree;
+      ps_dy_as_tokens_is_valid pre st.tokens;
+      serialize_parse_inv_lemma (bare_treesync_state tkt) session;
+      serialize_pre_lemma (bare_treesync_state tkt) pre st
+    )
+#pop-options
+
+val has_treesync_public_state_invariant: treekem_types dy_bytes -> preds -> prop
+let has_treesync_public_state_invariant tkt pr =
+  has_session_pred pr treesync_public_state_label (treesync_public_state_invariant tkt)
+
+(*** LCrypto API for public state ***)
+
+val treesync_state_to_session_bytes:
+  #tkt:treekem_types dy_bytes ->
+  pr:preds -> p:principal -> time:timestamp -> si:nat -> vi:nat ->
+  st:treesync_state dy_bytes tkt (dy_asp pr.global_usage time) ->
+  Pure dy_bytes
+  (requires
+    is_publishable pr.global_usage time st.group_id /\
+    treesync_has_pre (is_publishable pr.global_usage time) st.tree /\
+    (ps_dy_as_tokens st.levels 0).is_valid (is_publishable pr.global_usage time) st.tokens /\
+    has_treesync_public_state_invariant tkt pr
+  )
+  (ensures fun res -> treesync_public_state_invariant tkt pr.global_usage p time si vi res)
+let treesync_state_to_session_bytes #tkt pr p time si vi st =
+  let bare_st: bare_treesync_state tkt = {
+    group_id = st.group_id;
+    levels = st.levels;
+    tree = st.tree;
+    tokens = st.tokens;
+  } in
+  parse_serialize_inv_lemma #dy_bytes (bare_treesync_state tkt) bare_st;
+  serialize (bare_treesync_state tkt) bare_st
+
+val new_public_treesync_state:
+  #tkt:treekem_types dy_bytes ->
+  pr:preds -> p:principal -> time:timestamp ->
+  st:treesync_state dy_bytes tkt (dy_asp pr.global_usage time) ->
+  LCrypto nat pr
+  (requires fun t0 ->
+    time == trace_len t0 /\
+    is_publishable pr.global_usage time st.group_id /\
+    treesync_has_pre (is_publishable pr.global_usage time) st.tree /\
+    (ps_dy_as_tokens st.levels 0).is_valid (is_publishable pr.global_usage time) st.tokens /\
+    has_treesync_public_state_invariant tkt pr
+  )
+  (ensures fun t0 si t1 -> trace_len t1 == trace_len t0 + 1)
+let new_public_treesync_state #tkt pr p time st =
+  let si = new_session_number pr p in
+  let bare_st_bytes = treesync_state_to_session_bytes pr p time si 0 st in
+  new_session pr treesync_public_state_label (treesync_public_state_invariant tkt) p si 0 bare_st_bytes;
+  si
+
+val set_public_treesync_state:
+  #tkt:treekem_types dy_bytes ->
+  pr:preds -> p:principal -> si:nat -> time:timestamp ->
+  st:treesync_state dy_bytes tkt (dy_asp pr.global_usage time) ->
+  LCrypto unit pr
+  (requires fun t0 ->
+    time == trace_len t0 /\
+    is_publishable pr.global_usage time st.group_id /\
+    treesync_has_pre (is_publishable pr.global_usage time) st.tree /\
+    (ps_dy_as_tokens st.levels 0).is_valid (is_publishable pr.global_usage time) st.tokens /\
+    has_treesync_public_state_invariant tkt pr
+  )
+  (ensures fun t0 r t1 -> trace_len t1 == trace_len t0 + 1)
+let set_public_treesync_state #tkt pr p si time st =
+  let bare_st_bytes = treesync_state_to_session_bytes pr p time si 0 st in
+  update_session pr treesync_public_state_label (treesync_public_state_invariant tkt) p si 0 bare_st_bytes
+
+val get_public_treesync_state:
+  #tkt:treekem_types dy_bytes ->
+  pr:preds -> p:principal -> si:nat -> time:timestamp ->
+  LCrypto (treesync_state dy_bytes tkt (dy_asp pr.global_usage time)) pr
+  (requires fun t0 ->
+    time == trace_len t0 /\
+    has_treesync_public_state_invariant tkt pr
+  )
+  (ensures fun t0 st t1 ->
+    is_publishable pr.global_usage time st.group_id /\
+    treesync_has_pre (is_publishable pr.global_usage time) st.tree /\
+    t1 == t0
+  )
+let get_public_treesync_state #tkt pr p si time =
+  let (_, st_bytes) = get_session pr treesync_public_state_label (treesync_public_state_invariant tkt) p si in
+  let st = Some?.v (parse (bare_treesync_state tkt) st_bytes) in
+  {
+    group_id = st.group_id;
+    levels = st.levels;
+    tree = st.tree;
+    tokens = st.tokens;
+  }
+
+(*** Session predicate for private state ***)
+
+type treesync_private_state_ (bytes:Type0) {|bytes_like bytes|} = {
+  signature_key: mls_bytes bytes;
+}
+
+%splice [ps_treesync_private_state_] (gen_parser (`treesync_private_state_))
+%splice [ps_treesync_private_state__is_valid] (gen_is_valid_lemma (`treesync_private_state_))
+
+type treesync_private_state = treesync_private_state_ dy_bytes
+
+instance parseable_serializeable_treesync_private_state: parseable_serializeable dy_bytes treesync_private_state = mk_parseable_serializeable ps_treesync_private_state_
+
+val treesync_private_state_label: string
+let treesync_private_state_label = "MLS.TreeSync.PrivateState"
+
+val bare_treesync_private_state_invariant: bare_session_pred
+let bare_treesync_private_state_invariant gu p time si vi session =
+  match parse treesync_private_state session with
+  | None -> False
+  | Some st ->
+    is_signature_key gu "MLS.LeafSignKey" (readers [p_id p]) time st.signature_key
+
+val treesync_private_state_invariant: session_pred
+let treesync_private_state_invariant =
+  mk_session_pred bare_treesync_private_state_invariant
+    (fun gu p time0 time1 si vi session -> ())
+    (fun gu p time si vi session ->
+      let st = Some?.v (parse treesync_private_state session) in
+      let pre = is_msg gu (readers [psv_id p si vi]) time in
+      serialize_parse_inv_lemma treesync_private_state session;
+      serialize_pre_lemma treesync_private_state pre st
+    )
+
+val has_treesync_private_state_invariant: preds -> prop
+let has_treesync_private_state_invariant pr =
+  has_session_pred pr treesync_private_state_label treesync_private_state_invariant
+
+(*** LCrypto API for private state ***)
+
+val new_private_treesync_state:
+  pr:preds -> p:principal ->
+  st:treesync_private_state ->
+  LCrypto nat pr
+  (requires fun t0 ->
+    is_signature_key pr.global_usage "MLS.LeafSignKey" (readers [p_id p]) (trace_len t0) st.signature_key /\
+    has_treesync_private_state_invariant pr
+  )
+  (ensures fun t0 si t1 -> trace_len t1 == trace_len t0 + 1)
+let new_private_treesync_state pr p st =
+  let si = new_session_number pr p in
+  let st_bytes = serialize treesync_private_state st in
+  parse_serialize_inv_lemma #dy_bytes treesync_private_state st;
+  new_session pr treesync_private_state_label treesync_private_state_invariant p si 0 st_bytes;
+  si
+
+val set_private_treesync_state:
+  pr:preds -> p:principal -> si:nat ->
+  st:treesync_private_state ->
+  LCrypto unit pr
+  (requires fun t0 ->
+    is_signature_key pr.global_usage "MLS.LeafSignKey" (readers [p_id p]) (trace_len t0) st.signature_key /\
+    has_treesync_private_state_invariant pr
+  )
+  (ensures fun t0 r t1 -> trace_len t1 == trace_len t0 + 1)
+let set_private_treesync_state pr p si st =
+  let st_bytes = serialize treesync_private_state st in
+  parse_serialize_inv_lemma #dy_bytes treesync_private_state st;
+  new_session pr treesync_private_state_label treesync_private_state_invariant p si 0 st_bytes
+
+val get_private_treesync_state:
+  pr:preds -> p:principal -> si:nat ->
+  LCrypto treesync_private_state pr
+  (requires fun t0 -> has_treesync_private_state_invariant pr)
+  (ensures fun t0 st t1 ->
+    is_signature_key pr.global_usage "MLS.LeafSignKey" (readers [p_id p]) (trace_len t0) st.signature_key /\
+    t1 == t0
+  )
+let get_private_treesync_state pr p si =
+  let (_, st_bytes) = get_session pr treesync_private_state_label treesync_private_state_invariant p si in
+  let st = Some?.v (parse treesync_private_state st_bytes) in
+  st
